improved examples

LeanCourse/Examples.lean
@@ -18,7 +18,9 @@ def StorageT  := Value Nat ValueSelector valSelector
 def StateType := State Nat ValueSelector valSelector IdType
 def Selector  := FieldSelector ValueSelector valSelector
 def IdTyp     := IdT  ValueSelector valSelector IdType
-def ValSType   := ValT Nat ValueSelector valSelector IdType
+def ValSType  := ValT Nat ValueSelector valSelector IdType
+
+variable (mem : MemT) (st : StorageT)
 
 open Value
 open Memory
@@ -28,28 +30,40 @@ open Sum
 @[simp] def balance : Selector := .valS balanceS
 
 -- alice.account.balance = 10
-@[simp] def stAlice : StorageT := store mtst account $ store mtst balance $ var 10
-@[simp] def stBob   : StorageT := store mtst account $ store mtst balance $ var 20
+@[simp] def stAlice : StorageT := store st account $ store mtst balance $ var 10
+@[simp] def stBob   : StorageT := store st account $ store mtst balance $ var 20
 -- idA = alice
-@[simp] def memAlice (mem : MemT) := copySt mem idA stAlice
+@[simp] def memAlice (_ : isStruct st := by aesop) := copySt mem idA (stAlice st) $ by aesop
 
-theorem readCopy (mem : MemT) : Memory.read (memAlice mem) ⟨idA, [account]⟩ balance = .val 10
+theorem readCopy (_ : isStruct st := by aesop) : Memory.read (memAlice mem st) ⟨idA, [account]⟩ balance = .val 10
  := by simp
 
-@[simp] def memBob (mem : MemT) := copySt (memAlice mem) idB stBob
-@[simp] def idAA (mem : MemT) := read (memBob mem) ⟨idA, []⟩ account
-@[simp] def idBB (mem : MemT) := read (memBob mem) ⟨idB, []⟩ account
+@[simp] def memBob (_ : isStruct st := by aesop) := copySt (memAlice mem st) idB (stBob st) $ by aesop
+@[simp] def idAA (_ : isStruct st := by aesop) := read (memBob mem st) ⟨idA, []⟩ account
+@[simp] def idBB (_ : isStruct st := by aesop) := read (memBob mem st) ⟨idB, []⟩ account
 
-theorem readIdAA (mem : MemT) : idAA mem = .id ⟨idA, [account]⟩ := by simp
-theorem readIdBB (mem : MemT) : idBB mem = .id ⟨idB, [account]⟩ := by simp
+theorem readIdAA (_ : isStruct st := by aesop) : idAA mem st = .id ⟨idA, [account]⟩ := by simp
+theorem readIdBB (_ : isStruct st := by aesop) : idBB mem st = .id ⟨idB, [account]⟩ := by simp
 
-theorem readIdABalance (mem : MemT) : read (memBob mem) ⟨idA, [account]⟩ balance = .val 10  := by simp
+-- theorem readIdABalance (_ : isStruct st := by aesop) : read (memBob mem st) ⟨idA, [account]⟩ balance = .val 10  := by
+--   unfold memBob
+--   -- simp only [readSkip]
+--   have h := readFind mem idB st [account] balanceS $ by aesop
 
-theorem readIdBBalance (mem : MemT) : read (memBob mem) ⟨idB, [account]⟩ balance = .val 20  := by simp
+--   cases h with
+--   | mk _ _ => sorry
+--   | mkEmpty _ _ => sorry
+  -- . sorry
+  -- . sorry
+  -- sorry
+  -- rewrite [ ]
+  -- simp only [readSkip, readFind, skipIdRead, readGetId]
 
--- acc.balance = n
+theorem readIdBBalance (_ : isStruct st := by aesop) : read (memBob mem st) ⟨idB, [account]⟩ balance = .val 20  := by simp
+
+-- -- acc.balance = n
 @[simp] def stAcc (n : Nat) : StorageT := store mtst balance $ var n
--- idAcc = acc
+-- -- idAcc = acc
 @[simp] def memAcc (mem : MemT) (n : Nat) := copySt mem idAcc (stAcc n)
 
 theorem readAcc (mem : MemT) (n : Nat) : read (memAcc mem n) ⟨idAcc, []⟩ balance = .val n := by simp
